Added Machine.v

src/Step.v
@@ -1,58 +1,31 @@
 Require Import
-  Program
-  Coq.Lists.List
-  Coq.Relations.Relation_Definitions
-  Coq.Classes.Equivalence
+  Coq.Program.Program
   Coq.Classes.Morphisms
-  Coq.Classes.RelationClasses
-  Coq.Logic.Classical
-  Coq.Sets.Ensembles.
+  Coq.Lists.List
+  Syntax.
 
 Open Scope program_scope.
-Open Scope list_scope.
 
-Require Import LTL.
+Module LTLStep (S : StreamType).
 
-Generalizable All Variables.
-Set Transparent Obligations.
-Set Decidable Equality Schemes.
-
-Section Step.
-
-Variable a : Type.              (* The type of entries in the trace *)
+Module Import LTL := LTL S.
 
 Inductive Failed : Type :=
   | HitBottom
   | EndOfTrace
-  | Rejected    (x : a)
+  | Rejected    (x : S.a)
   | BothFailed  (p q : Failed)
   | LeftFailed  (p : Failed)
   | RightFailed (q : Failed).
 
 Inductive Result : Type :=
-  (* | Ask (f : a -> Result) *)
   | Failure (e : Failed)
-  | Continue (l : LTL a)
+  | Continue (l : Formula)
   | Success.
-
-(*
-Definition frob `(f : Eff A) : Eff A :=
-  match f with
-  | Stop x  => Stop x
-  | Delay m => Delay m
-  | Repeat  => Repeat
-  | Ask k   => Ask k
-  end.
-
-Theorem frob_eq : forall A (f : Eff A), f = frob f.
-Proof. destruct f; reflexivity. Qed.
-*)
 
 Open Scope ltl_scope.
 
-Arguments expand {_} _.
-
-Definition and (f g : Result) : Result :=
+Definition and_result (f g : Result) : Result :=
   match f, g with
   | Failure e, _   => Failure (LeftFailed e)
   | _, Failure e   => Failure (RightFailed e)
@@ -60,12 +33,9 @@ Definition and (f g : Result) : Result :=
     Continue g'    => Continue (f' ∧ g')
   | f', Success    => f'
   | Success, g'    => g'
-  (* | Ask f', Ask g' => Ask (fun a => and (f' a) (g' a)) *)
-  (* | f', Ask g'     => Ask (fun a => and f' (g' a)) *)
-  (* | Ask f', g'     => Ask (fun a => and (f' a) g') *)
   end.
 
-Definition or (f g : Result) : Result :=
+Definition or_result (f g : Result) : Result :=
   match f, g with
   | Failure e1,
     Failure e2     => Failure (BothFailed e1 e2)
@@ -75,57 +45,83 @@ Definition or (f g : Result) : Result :=
     Continue g'    => Continue (f' ∨ g')
   | Failure _, g'  => g'
   | f', Failure _  => f'
-  (* | Ask f', Ask g' => Ask (fun a => and (f' a) (g' a)) *)
-  (* | f', Ask g'     => Ask (fun a => and f' (g' a)) *)
-  (* | Ask f', g'     => Ask (fun a => and (f' a) g') *)
   end.
 
-Fixpoint compile (l : LTL a) : option a -> Result := fun mx =>
+Fixpoint compile (l : Formula) : option S.a -> Result := fun mx =>
   match l with
-  | ⊤ => Success
-  | ⊥ => Failure HitBottom
+  | Top    => Success
+  | Bottom => Failure HitBottom
 
-  | Accept v =>
+  | Examine v =>
     match mx with
-    | None   => Success
-    | Some x => compile (v x) (Some x)
+    | None   => compile (v None) None
+    | Some x => compile (v (Some x)) (Some x)
     end
 
-  | p ∧ q => and (compile p mx) (compile q mx)
-  | p ∨ q => or  (compile p mx) (compile q mx)
+  | And p q => and_result (compile p mx) (compile q mx)
+  | Or p q  => or_result (compile p mx) (compile q mx)
 
-  | X p   =>
+  | Next p   =>
     match mx with
     | None   => compile p None
     | Some _ => Continue p
     end
 
-  | p U q =>
+  | Until p q =>
     match mx with
     | None   => compile q None
-    | Some x => or (compile q mx) (and (compile p mx) (Continue (p U q)))
+    | Some x => or_result (compile q mx)
+                          (and_result (compile p mx) (Continue (Until p q)))
     end
 
-  | p R q =>
+  | Release p q =>
     match mx with
     | None   => compile q None
-    | Some x => and (compile q mx) (or (compile p mx) (Continue (p R q)))
+    | Some x => and_result (compile q mx)
+                           (or_result (compile p mx) (Continue (Release p q)))
+    end
+
+  | Always p =>
+    match mx with
+    | None   => compile p None
+    | Some x => and_result (compile p mx) (Continue (Always p))
+    end
+
+  | Eventually p =>
+    match mx with
+    | None   => compile p None
+    | Some x => or_result (compile p mx) (Continue (Eventually p))
+    end
+
+  | Wait p q =>
+    match mx with
+    | None   => or_result (compile q None) (compile p None)
+    | Some x => or_result (compile q mx)
+                          (and_result (compile p mx) (Continue (Wait p q)))
+    end
+
+  | StrongRelease p q =>
+    match mx with
+    | None   => and_result (compile q None) (compile p None)
+    | Some x => and_result (compile q mx)
+                           (or_result (compile p mx) (Continue (StrongRelease p q)))
     end
   end.
 
-Definition step (m : Result) (x : a) : Result :=
+Definition step (m : Result) (x : S.a) : Result :=
   match m with
   | Continue l => compile l (Some x)
   | r => r
   end.
 
-Function run (m : LTL a) (xs : list a) : Result :=
+Function run (m : Formula) (xs : list S.a) : Result :=
   match xs with
-  | []      => compile m None
+  | nil     => compile m None
   | x :: xs =>
     match compile m (Some x) with
     | Continue l => run l xs
-    | r => r
+    | Failure e  => Failure e
+    | Success    => Success
     end
   end.
 
@@ -136,8 +132,7 @@ Definition passes (r : Result) : Prop :=
   | Success    => True
   end.
 
-Definition passes_equiv (p q : Result) : Prop :=
-  passes p <-> passes q.
+Definition passes_equiv (p q : Result) : Prop := passes p <-> passes q.
 Arguments passes_equiv p q /.
 
 Global Program Instance Equivalence_passes_equiv : Equivalence passes_equiv.
@@ -155,145 +150,320 @@ Next Obligation.
   repeat intro; firstorder.
 Qed.
 
-Lemma run_and p q xs :
-  passes (run (p ∧ q) xs) <-> passes (run p xs) /\ passes (run q xs).
+Lemma run_and p q s :
+  passes (run (p ∧ q) s) <-> passes (run p s) /\ passes (run q s).
 Proof.
-  generalize dependent p.
-  generalize dependent q.
-  induction xs; simpl; intros;
-  intuition auto;
-  try destruct (compile p Nothing) eqn:?;
-  try destruct (compile q Nothing) eqn:?;
-  try destruct (compile p (Some a0)) eqn:?;
-  try destruct (compile q (Some a0)) eqn:?;
-  try specialize (proj1 (IHxs _ _) H); intros;
-  simpl in *; now intuition.
+  unfold and.
+  split; intros.
+  - generalize dependent p.
+    generalize dependent q.
+    induction s; simpl; intros; intuition.
+    + destruct (compile p None); simpl in *; intuition.
+    + destruct (compile q None); simpl in *; intuition.
+      destruct (compile p None); simpl in *; intuition.
+    + destruct (compile p (Some a)) eqn:?; simpl in *; intuition.
+      destruct (compile q (Some a)) eqn:?; simpl in *; intuition.
+      now specialize (IHs _ _ H).
+    + destruct (compile p (Some a)) eqn:?; simpl in *; intuition;
+      destruct (compile q (Some a)) eqn:?; simpl in *; intuition.
+      now specialize (IHs _ _ H).
+  - generalize dependent p.
+    generalize dependent q.
+    induction s; simpl; intros; intuition.
+    + destruct (compile p None) eqn:?; simpl in *; intuition;
+      destruct (compile q None) eqn:?; simpl in *; intuition.
+    + destruct (compile p (Some a)) eqn:?; simpl in *; intuition;
+      destruct (compile q (Some a)) eqn:?; simpl in *; intuition.
 Qed.
 
-Lemma run_or p q xs :
-  passes (run (p ∨ q) xs) <-> passes (run p xs) \/ passes (run q xs).
+Lemma run_or p q s :
+  passes (run (p ∨ q) s) <-> passes (run p s) \/ passes (run q s).
 Proof.
-  generalize dependent p.
-  generalize dependent q.
-  induction xs; simpl; intros;
-  intuition auto;
-  try destruct (compile p Nothing) eqn:?;
-  try destruct (compile q Nothing) eqn:?;
-  try destruct (compile p (Some a0)) eqn:?;
-  try destruct (compile q (Some a0)) eqn:?;
-  try specialize (proj1 (IHxs _ _) H); intros;
-  simpl in *; now intuition.
+  unfold and.
+  split; intros.
+  - generalize dependent p.
+    generalize dependent q.
+    induction s; simpl; intros; intuition.
+    + destruct (compile p None); simpl in *; intuition;
+      destruct (compile q None); simpl in *; intuition.
+    + destruct (compile p (Some a)) eqn:?; simpl in *; intuition;
+      destruct (compile q (Some a)) eqn:?; simpl in *; intuition.
+  - generalize dependent p.
+    generalize dependent q.
+    induction s; simpl; intros; intuition.
+    + destruct (compile p None) eqn:?; simpl in *; intuition;
+      destruct (compile q None) eqn:?; simpl in *; intuition.
+    + destruct (compile p None) eqn:?; simpl in *; intuition;
+      destruct (compile q None) eqn:?; simpl in *; intuition.
+    + destruct (compile p (Some a)) eqn:?; simpl in *; intuition;
+      destruct (compile q (Some a)) eqn:?; simpl in *; intuition.
+    + destruct (compile p (Some a)) eqn:?; simpl in *; intuition;
+      destruct (compile q (Some a)) eqn:?; simpl in *; intuition.
 Qed.
 
 Lemma run_next p x xs :
-  passes (run (X p) (x :: xs)) <-> passes (run p xs).
+  passes (run (Next p) (x :: xs)) <-> passes (run p xs).
 Proof. now induction xs; intuition. Qed.
 
 Lemma run_until p q s :
-  passes (run (p U q) s) <->
+  passes (run (Until p q) s) <->
   let fix go s :=
       match s with
-      | [] => passes (run q s)
+      | nil     => passes (run q s)
       | _ :: xs => passes (run q s) \/ (passes (run p s) /\ go xs)
       end in go s.
 Proof.
-  generalize dependent p.
-  generalize dependent q.
-  induction s; simpl; intros.
-  - split; auto.
-  - destruct (compile p (Some a0)) eqn:?;
-    destruct (compile q (Some a0)) eqn:?; simpl;
-    intuition auto.
-    + apply run_and in H.
-      intuition.
-    + apply IHs in H1.
-      apply run_and; auto.
-    + apply run_or in H.
-      destruct H; auto.
-      apply run_and in H.
-      intuition.
-    + apply run_or.
-      intuition.
-    + apply IHs in H1.
-      apply run_or; intuition.
-      right.
-      apply run_and; auto.
-    + right.
-      split; auto.
-      now apply IHs.
-    + now apply IHs in H1.
-    + apply run_or in H.
-      intuition.
-    + apply run_or.
-      intuition.
-    + apply IHs in H1.
-      apply run_or.
-      intuition.
+  unfold and.
+  split; intros.
+  - generalize dependent p.
+    generalize dependent q.
+    induction s; simpl; intros; intuition.
+    destruct (compile p (Some a)) eqn:?; simpl in *; intuition;
+    destruct (compile q (Some a)) eqn:?; simpl in *; intuition.
+    + rewrite run_and in H.
+      now firstorder.
+    + rewrite run_or, run_and in H.
+      now firstorder.
+    + now firstorder.
+    + rewrite run_or in H.
+      now firstorder.
+  - generalize dependent p.
+    generalize dependent q.
+    induction s; simpl; intros; intuition.
+    destruct (compile p (Some a)) eqn:?; simpl in *; intuition;
+    destruct (compile q (Some a)) eqn:?; simpl in *; intuition.
+    + rewrite run_or, run_and.
+      now firstorder.
+    + rewrite run_or.
+      now firstorder.
+    + destruct (compile p (Some a)) eqn:?; simpl in *; intuition;
+      destruct (compile q (Some a)) eqn:?; simpl in *; intuition.
+      * rewrite run_and.
+        now firstorder.
+      * rewrite run_or, run_and.
+        now firstorder.
+      * rewrite run_or.
+        now firstorder.
+Qed.
+
+Lemma run_wait p q s :
+  passes (run (Wait p q) s) <->
+  let fix go s :=
+      match s with
+      | nil     => passes (run q s) \/ passes (run p s)
+      | _ :: xs => passes (run q s) \/ (passes (run p s) /\ go xs)
+      end in go s.
+Proof.
+  unfold and.
+  split; intros.
+  - generalize dependent p.
+    generalize dependent q.
+    induction s; simpl; intros; intuition.
+    + destruct (compile p None) eqn:?; simpl in *; intuition;
+      destruct (compile q None) eqn:?; simpl in *; intuition.
+    + destruct (compile p (Some a)) eqn:?; simpl in *; intuition;
+      destruct (compile q (Some a)) eqn:?; simpl in *; intuition.
+      * rewrite run_and in H.
+        now firstorder.
+      * rewrite run_or, run_and in H.
+        now firstorder.
+      * now firstorder.
+      * rewrite run_or in H.
+        now firstorder.
+  - generalize dependent p.
+    generalize dependent q.
+    induction s; simpl; intros; intuition.
+    + destruct (compile p None) eqn:?; simpl in *; intuition;
+      destruct (compile q None) eqn:?; simpl in *; intuition.
+    + destruct (compile p None) eqn:?; simpl in *; intuition;
+      destruct (compile q None) eqn:?; simpl in *; intuition.
+    + destruct (compile p (Some a)) eqn:?; simpl in *; intuition;
+      destruct (compile q (Some a)) eqn:?; simpl in *; intuition.
+      * rewrite run_or, run_and.
+        now firstorder.
+      * rewrite run_or.
+        now firstorder.
+    + destruct (compile p (Some a)) eqn:?; simpl in *; intuition;
+      destruct (compile q (Some a)) eqn:?; simpl in *; intuition.
+      * rewrite run_and.
+        now firstorder.
+      * rewrite run_or, run_and.
+        now firstorder.
+      * rewrite run_or.
+        now firstorder.
+Qed.
+
+Lemma run_always p s :
+  passes (run (Always p) s) <->
+  let fix go s :=
+      match s with
+      | nil     => passes (run p s)
+      | _ :: xs => passes (run p s) /\ go xs
+      end in go s.
+Proof.
+  unfold and.
+  split; intros.
+  - generalize dependent p.
+    induction s; simpl; intros; intuition.
+    + destruct (compile p (Some a)) eqn:?; simpl in *; intuition.
+      rewrite run_and in H.
+      now firstorder.
+    + destruct (compile p (Some a)) eqn:?; simpl in *; intuition.
+      * rewrite run_and in H.
+        now firstorder.
+      * now firstorder.
+  - generalize dependent p.
+    induction s; simpl; intros; intuition.
+    destruct (compile p (Some a)) eqn:?; simpl in *; intuition.
+    rewrite run_and.
+    now firstorder.
+Qed.
+
+Lemma run_eventually p s :
+  passes (run (Eventually p) s) <->
+  let fix go s :=
+      match s with
+      | nil     => passes (run p s)
+      | _ :: xs => passes (run p s) \/ go xs
+      end in go s.
+Proof.
+  unfold and.
+  split; intros.
+  - generalize dependent p.
+    induction s; simpl; intros; intuition.
+    + destruct (compile p (Some a)) eqn:?; simpl in *; intuition.
+      * now firstorder.
+      * rewrite run_or in H.
+        now firstorder.
+  - generalize dependent p.
+    induction s; simpl; intros; intuition.
+    + destruct (compile p (Some a)) eqn:?; simpl in *; intuition.
+      rewrite run_or.
+      now firstorder.
+    + destruct (compile p (Some a)) eqn:?; simpl in *; intuition.
+      rewrite run_or.
+      now firstorder.
 Qed.
 
 Lemma run_release p q s :
-  passes (run (p R q) s) <->
+  passes (run (Release p q) s) <->
   let fix go s :=
       match s with
-      | [] => passes (run q s)
+      | nil     => passes (run q s)
       | _ :: xs => passes (run q s) /\ (passes (run p s) \/ go xs)
       end in go s.
 Proof.
-  generalize dependent p.
-  generalize dependent q.
-  induction s; intros.
-  - now intuition.
-  - simpl; split; intros;
-    destruct (compile p (Some a0)) eqn:?;
-    destruct (compile q (Some a0)) eqn:?; simpl in *;
-    intuition auto.
-    + apply run_and in H.
-      now intuition.
-    + apply run_and in H.
-      now intuition.
-    + apply IHs in H.
-      now right.
-    + apply run_and in H.
-      now intuition.
-    + apply run_and in H.
-      destruct H.
-      apply run_or in H0.
-      now intuition.
-    + apply run_or in H.
-      now intuition.
-    + apply run_and.
-      now intuition.
-    + now apply IHs.
-    + apply run_and.
-      split; auto.
-      apply run_or.
-      now intuition.
-    + apply run_and.
-      split; auto.
-      apply run_or.
-      now intuition.
-    + apply run_or.
-      now intuition.
-    + apply run_or.
-      now intuition.
+  unfold and.
+  split; intros.
+  - generalize dependent p.
+    generalize dependent q.
+    induction s; simpl; intros; intuition.
+    destruct (compile p (Some a)) eqn:?; simpl in *; intuition;
+    destruct (compile q (Some a)) eqn:?; simpl in *; intuition.
+    + rewrite run_and in H.
+      now firstorder.
+    + rewrite run_and, run_or in H.
+      now firstorder.
+    + destruct (compile p (Some a)) eqn:?; simpl in *; intuition;
+      destruct (compile q (Some a)) eqn:?; simpl in *; intuition.
+      * rewrite run_and in H.
+        now firstorder.
+      * now firstorder.
+      * rewrite run_and, run_or in H.
+        now firstorder.
+      * rewrite run_or in H.
+        now firstorder.
+  - generalize dependent p.
+    generalize dependent q.
+    induction s; simpl; intros; intuition.
+    destruct (compile p (Some a)) eqn:?; simpl in *; intuition;
+    destruct (compile q (Some a)) eqn:?; simpl in *; intuition.
+    + rewrite run_and, run_or.
+      now firstorder.
+    + rewrite run_or.
+      now firstorder.
+    + destruct (compile p (Some a)) eqn:?; simpl in *; intuition;
+      destruct (compile q (Some a)) eqn:?; simpl in *; intuition.
+      * rewrite run_and.
+        now firstorder.
+      * rewrite run_and, run_or.
+        now firstorder.
+      * rewrite run_or.
+        now firstorder.
 Qed.
 
-Lemma run_correct (l : LTL a) (s : Stream a) :
-  matches a l s <-> passes (run l s).
+Lemma run_strong_release p q s :
+  passes (run (StrongRelease p q) s) <->
+  let fix go s :=
+      match s with
+      | nil     => passes (run q s) /\ passes (run p s)
+      | _ :: xs => passes (run q s) /\ (passes (run p s) \/ go xs)
+      end in go s.
+Proof.
+  unfold and.
+  split; intros.
+  - generalize dependent p.
+    generalize dependent q.
+    induction s; simpl; intros; intuition.
+    + destruct (compile p None) eqn:?; simpl in *; intuition;
+      destruct (compile q None) eqn:?; simpl in *; intuition.
+    + destruct (compile p None) eqn:?; simpl in *; intuition;
+      destruct (compile q None) eqn:?; simpl in *; intuition.
+    + destruct (compile p (Some a)) eqn:?; simpl in *; intuition;
+      destruct (compile q (Some a)) eqn:?; simpl in *; intuition.
+      * rewrite run_and in H.
+        now firstorder.
+      * rewrite run_and, run_or in H.
+        now firstorder.
+    + destruct (compile p (Some a)) eqn:?; simpl in *; intuition;
+      destruct (compile q (Some a)) eqn:?; simpl in *; intuition.
+      * rewrite run_and in H.
+        now firstorder.
+      * now firstorder.
+      * rewrite run_and, run_or in H.
+        now firstorder.
+      * rewrite run_or in H.
+        now firstorder.
+  - generalize dependent p.
+    generalize dependent q.
+    induction s; simpl; intros; intuition.
+    + destruct (compile p None) eqn:?; simpl in *; intuition;
+      destruct (compile q None) eqn:?; simpl in *; intuition.
+    + destruct (compile p (Some a)) eqn:?; simpl in *; intuition;
+      destruct (compile q (Some a)) eqn:?; simpl in *; intuition.
+      * rewrite run_and, run_or.
+        now firstorder.
+      * rewrite run_or.
+        now firstorder.
+    + destruct (compile p (Some a)) eqn:?; simpl in *; intuition;
+      destruct (compile q (Some a)) eqn:?; simpl in *; intuition.
+      * rewrite run_and.
+        now firstorder.
+      * rewrite run_and, run_or.
+        now firstorder.
+      * rewrite run_or.
+        now firstorder.
+Qed.
+
+Lemma run_correct (l : Formula) (s : list S.a) :
+  matches l s <-> passes (run l s).
 Proof.
   generalize dependent s.
-  induction l; simpl; intros.
+  induction l; intros.
   - now induction s.
   - now induction s.
   - induction s; intuition.
-    now specialize (proj1 (H _ _) H2).
+    + now specialize (proj1 (H _ _) H0).
+    + now apply H, H0.
+    + now specialize (proj1 (H _ _) H2).
+    + now apply H, H2.
   - split; intros.
       destruct H.
       specialize (proj1 (IHl1 _) H); intros; clear IHl1 H.
       specialize (proj1 (IHl2 _) H0); intros; clear IHl2 H0.
       now apply run_and.
     apply run_and in H.
-    now split; intuition.
+    now firstorder.
   - split; intros.
       destruct H.
         specialize (proj1 (IHl1 _) H); intros; clear IHl1 H.
@@ -303,38 +473,67 @@ Proof.
       apply run_or.
       now right.
     apply run_or in H.
-    now intuition.
+    now firstorder.
   - split; intros;
     induction s; intuition.
-    now apply IHl in H.
+    + now apply IHl in H.
+    + now apply IHl in H.
+    + now apply IHl.
+    + now apply IHl.
   - split; intros.
       apply run_until.
       simpl.
-      induction s; intuition.
+      now induction s; firstorder.
     apply run_until in H.
-    induction s; intuition.
+    now induction s; firstorder.
   - split; intros.
       apply run_release.
       simpl.
-      induction s; intuition.
+      now induction s; firstorder.
     apply run_release in H.
-    induction s; intuition.
+    now induction s; firstorder.
+  - split; intros.
+      apply run_always.
+      simpl.
+      now induction s; firstorder.
+    apply run_always in H.
+    now induction s; firstorder.
+  - split; intros.
+      apply run_eventually.
+      simpl.
+      now induction s; firstorder.
+    apply run_eventually in H.
+    now induction s; firstorder.
+  - split; intros.
+      apply run_wait.
+      simpl.
+      now induction s; firstorder.
+    apply run_wait in H.
+    now induction s; firstorder.
+  - split; intros.
+      apply run_strong_release.
+      simpl.
+      now induction s; firstorder.
+    apply run_strong_release in H.
+    now induction s; firstorder.
 Qed.
 
-End Step.
-
+(*
 Section Examples.
 
-Open Scope list_scope.
-Open Scope ltl_scope.
+Import ListNotations.
 
-Goal passes _ (run _ (□ (num 3 → X (num 4))) [2; 3; 4]).
+Open Scope list_scope.
+
+Goal passes _ (run _ (□ (num 3 ⇒ X (num 4))) [2; 3; 4]).
   simpl.
 Abort.
 
-Goal passes _ (run _ (□ (num 3 → ◇ (num 8)))
-                     [1; 2; 3; 4; 5; 6; 7; 8; 9]).
+Goal passes _ (run _ (□ (num 3 ⇒ ◇ (num 8))) [1; 2; 3; 4; 5; 6; 7; 8; 9]).
   simpl.
 Abort.
 
 End Examples.
+*)
+
+End LTLStep.
