src/Machine.v
@@ -1,0 +1,149 @@
+Require Import
+  Coq.Program.Program
+  Coq.Unicode.Utf8
+  Coq.Classes.Morphisms
+  Coq.Lists.List
+  Syntax.
+
+Open Scope program_scope.
+
+CoInductive Machine (a b : Type) :=
+  | Step : (a -> Machine a b + b) -> Machine a b.
+
+Arguments Step {a b} _.
+
+CoFixpoint map {a b c : Type} (f : b -> c) (p : Machine a b) : Machine a c :=
+  match p with
+  | Step k => Step (λ x, match k x with
+                         | inl m => inl (map f m)
+                         | inr r => inr (f r)
+                         end)
+  end.
+
+Module LTLMachine (S : StreamType).
+
+Module Import LTL := LTL S.
+
+Inductive Failed : Type :=
+  | HitBottom
+  | Rejected    (x : S.a)
+  | BothFailed  (p q : Failed)
+  | LeftFailed  (p : Failed)
+  | RightFailed (q : Failed).
+
+Inductive Result : Type :=
+  | Failure (e : Failed)
+  | Success.
+
+Definition LTL := Machine S.a Result.
+
+Definition stop (r : Result) : LTL := Step (λ _, inr r).
+
+Definition true := stop Success.
+
+Definition false := stop (Failure HitBottom).
+
+Definition invert (r : Result) : Result :=
+  match r with
+  | Failure e => Success
+  | Success   => Failure HitBottom
+  end.
+
+Definition negate : LTL -> LTL := map invert.
+
+Definition next (p : LTL) : LTL :=
+  match p with
+  | Step k => Step (λ _, inl (Step k))
+  end.
+
+CoFixpoint and (p q : LTL) : LTL :=
+  match p with
+  | Step k =>
+    Step (λ a,
+          match k a with
+          | inr (Failure e) => inr (Failure (LeftFailed e))
+          | inr Success     =>
+            match q with
+            | Step g => g a
+            end
+          | inl p' =>
+            match q with
+            | Step g =>
+              match g a with
+              | inr (Failure e) => inr (Failure (RightFailed e))
+              | inr Success     => inl p'
+              | inl q'          => inl (and p' q')
+              end
+            end
+          end)
+  end.
+
+Definition andNext (p q : LTL) : LTL :=
+  match p with
+  | Step k =>
+    Step (λ a,
+          match k a with
+          | inr (Failure e) => inr (Failure (LeftFailed e))
+          | inr Success     => inl q
+          | inl p'          => inl (and p' q)
+          end)
+  end.
+
+CoFixpoint or (p q : LTL) : LTL :=
+  match p with
+  | Step k =>
+    Step (λ a,
+          match k a with
+          | inr Success      => inr Success
+          | inr (Failure e1) =>
+            match q with
+            | Step g =>
+              match g a with
+              | inr (Failure e2) => inr (Failure (BothFailed e1 e2))
+              | q' => q'
+              end
+            end
+          | inl p' =>
+            match q with
+            | Step g =>
+              match g a with
+              | inr Success     => inr Success
+              | inr (Failure _) => inl p'
+              | inl q'          => inl (or p' q')
+              end
+            end
+          end)
+  end.
+
+Definition orNext (p q : LTL) : LTL :=
+  match p with
+  | Step k =>
+    Step (λ a,
+          match k a with
+          | inr Success     => inr Success
+          | inr (Failure _) => inl q
+          | inl p'          => inl (or p' q)
+          end)
+  end.
+
+(*
+CoFixpoint until (p q : LTL) : LTL :=
+  or q (andNext p (until p q)).
+
+CoFixpoint wait (p q : LTL) : LTL :=
+  or q (andNext p (wait p q)).
+
+CoFixpoint always (p : LTL) : LTL :=
+  andNext p (always p).
+
+CoFixpoint eventually (p : LTL) : LTL :=
+  orNext p (eventually p).
+
+CoFixpoint release (p q : LTL) : LTL :=
+  and q (orNext p (release p q)).
+
+CoFixpoint strong_release (p q : LTL) : LTL :=
+  and q (orNext p (strong_release p q)).
+*)
+
+End LTLMachine.
